RocqOfNoir/keccak/polymorphic.v
@@ -5,40 +5,20 @@ Require Import keccak.monomorphic.
 (** This module provides helpers to show the equality to debug [reflexivity] when it is too long or
     failing *)
 Module Eq.
-  Lemma LowLet {A : Set} (e e' : LowM.t A) k k'
+  Lemma Let (e e' : M.t) k k'
       (H_e : e = e')
       (H_k : forall x, k x = k' x) :
-    LowM.Let e k = LowM.Let e' k'.
+    M.Let e k = M.Let e' k'.
   Proof.
     rewrite H_e.
     replace k with k' by now apply functional_extensionality.
     reflexivity.
   Qed.
 
-  Lemma LetMinus {A : Set} (e1 e1' : LowM.t A) (e2 e2' : A -> LowM.t A)
-      (H_e1 : e1 = e1')
-      (H_e2 : forall x, e2 x = e2' x) :
-    LowM.let_ e1 e2 = LowM.let_ e1' e2'.
-  Proof.
-    rewrite H_e1.
-    replace e2 with e2' by now apply functional_extensionality.
-    reflexivity.
-  Qed.
-
-  Lemma LetStar e1 e1' e2 e2'
+  Lemma LetMinus (e1 e1' : M.t) (e2 e2' : Value.t -> M.t)
       (H_e1 : e1 = e1')
       (H_e2 : forall x, e2 x = e2' x) :
     M.let_ e1 e2 = M.let_ e1' e2'.
-  Proof.
-    rewrite H_e1.
-    replace e2 with e2' by now apply functional_extensionality.
-    reflexivity.
-  Qed.
-
-  Lemma LetTilde e1 e1' e2 e2'
-      (H_e1 : e1 = e1')
-      (H_e2 : forall x, e2 x = e2' x) :
-    M.let_strong e1 e2 = M.let_strong e1' e2'.
   Proof.
     rewrite H_e1.
     replace e2 with e2' by now apply functional_extensionality.
@@ -57,13 +37,23 @@ Module Eq.
   Ltac tactic :=
     repeat (
       intro ||
-      apply LowLet ||
+      apply Let ||
       apply LetMinus ||
-      apply LetStar ||
-      apply LetTilde ||
       apply If
     ).
 End Eq.
+
+(* global BLOCK_SIZE_IN_BYTES: u32 = 136; *)
+Definition BLOCK_SIZE_IN_BYTES: Z := 136.
+
+(* global WORD_SIZE: u32 = 8; *)
+Definition WORD_SIZE: Z := 8.
+
+(* global LIMBS_PER_BLOCK: u32 = BLOCK_SIZE_IN_BYTES / WORD_SIZE; *)
+Definition LIMBS_PER_BLOCK: Z := BLOCK_SIZE_IN_BYTES / WORD_SIZE.
+
+(* global NUM_KECCAK_LANES: u32 = 25; *)
+Definition NUM_KECCAK_LANES: Z := 25.
 
 Definition keccak256 (N : U32.t) (α : list Value.t) : M.t :=
   match α with
@@ -81,144 +71,9 @@ Definition keccak256 (N : U32.t) (α : list Value.t) : M.t :=
         |))
       ]] in
       let~ block_bytes := [[ M.copy_mutable (|
-        M.alloc (Value.Array [
-          Value.Integer IntegerKind.U8 0;
-          Value.Integer IntegerKind.U8 0;
-          Value.Integer IntegerKind.U8 0;
-          Value.Integer IntegerKind.U8 0;
-          Value.Integer IntegerKind.U8 0;
-          Value.Integer IntegerKind.U8 0;
-          Value.Integer IntegerKind.U8 0;
-          Value.Integer IntegerKind.U8 0;
-          Value.Integer IntegerKind.U8 0;
-          Value.Integer IntegerKind.U8 0;
-          Value.Integer IntegerKind.U8 0;
-          Value.Integer IntegerKind.U8 0;
-          Value.Integer IntegerKind.U8 0;
-          Value.Integer IntegerKind.U8 0;
-          Value.Integer IntegerKind.U8 0;
-          Value.Integer IntegerKind.U8 0;
-          Value.Integer IntegerKind.U8 0;
-          Value.Integer IntegerKind.U8 0;
-          Value.Integer IntegerKind.U8 0;
-          Value.Integer IntegerKind.U8 0;
-          Value.Integer IntegerKind.U8 0;
-          Value.Integer IntegerKind.U8 0;
-          Value.Integer IntegerKind.U8 0;
-          Value.Integer IntegerKind.U8 0;
-          Value.Integer IntegerKind.U8 0;
-          Value.Integer IntegerKind.U8 0;
-          Value.Integer IntegerKind.U8 0;
-          Value.Integer IntegerKind.U8 0;
-          Value.Integer IntegerKind.U8 0;
-          Value.Integer IntegerKind.U8 0;
-          Value.Integer IntegerKind.U8 0;
-          Value.Integer IntegerKind.U8 0;
-          Value.Integer IntegerKind.U8 0;
-          Value.Integer IntegerKind.U8 0;
-          Value.Integer IntegerKind.U8 0;
-          Value.Integer IntegerKind.U8 0;
-          Value.Integer IntegerKind.U8 0;
-          Value.Integer IntegerKind.U8 0;
-          Value.Integer IntegerKind.U8 0;
-          Value.Integer IntegerKind.U8 0;
-          Value.Integer IntegerKind.U8 0;
-          Value.Integer IntegerKind.U8 0;
-          Value.Integer IntegerKind.U8 0;
-          Value.Integer IntegerKind.U8 0;
-          Value.Integer IntegerKind.U8 0;
-          Value.Integer IntegerKind.U8 0;
-          Value.Integer IntegerKind.U8 0;
-          Value.Integer IntegerKind.U8 0;
-          Value.Integer IntegerKind.U8 0;
-          Value.Integer IntegerKind.U8 0;
-          Value.Integer IntegerKind.U8 0;
-          Value.Integer IntegerKind.U8 0;
-          Value.Integer IntegerKind.U8 0;
-          Value.Integer IntegerKind.U8 0;
-          Value.Integer IntegerKind.U8 0;
-          Value.Integer IntegerKind.U8 0;
-          Value.Integer IntegerKind.U8 0;
-          Value.Integer IntegerKind.U8 0;
-          Value.Integer IntegerKind.U8 0;
-          Value.Integer IntegerKind.U8 0;
-          Value.Integer IntegerKind.U8 0;
-          Value.Integer IntegerKind.U8 0;
-          Value.Integer IntegerKind.U8 0;
-          Value.Integer IntegerKind.U8 0;
-          Value.Integer IntegerKind.U8 0;
-          Value.Integer IntegerKind.U8 0;
-          Value.Integer IntegerKind.U8 0;
-          Value.Integer IntegerKind.U8 0;
-          Value.Integer IntegerKind.U8 0;
-          Value.Integer IntegerKind.U8 0;
-          Value.Integer IntegerKind.U8 0;
-          Value.Integer IntegerKind.U8 0;
-          Value.Integer IntegerKind.U8 0;
-          Value.Integer IntegerKind.U8 0;
-          Value.Integer IntegerKind.U8 0;
-          Value.Integer IntegerKind.U8 0;
-          Value.Integer IntegerKind.U8 0;
-          Value.Integer IntegerKind.U8 0;
-          Value.Integer IntegerKind.U8 0;
-          Value.Integer IntegerKind.U8 0;
-          Value.Integer IntegerKind.U8 0;
-          Value.Integer IntegerKind.U8 0;
-          Value.Integer IntegerKind.U8 0;
-          Value.Integer IntegerKind.U8 0;
-          Value.Integer IntegerKind.U8 0;
-          Value.Integer IntegerKind.U8 0;
-          Value.Integer IntegerKind.U8 0;
-          Value.Integer IntegerKind.U8 0;
-          Value.Integer IntegerKind.U8 0;
-          Value.Integer IntegerKind.U8 0;
-          Value.Integer IntegerKind.U8 0;
-          Value.Integer IntegerKind.U8 0;
-          Value.Integer IntegerKind.U8 0;
-          Value.Integer IntegerKind.U8 0;
-          Value.Integer IntegerKind.U8 0;
-          Value.Integer IntegerKind.U8 0;
-          Value.Integer IntegerKind.U8 0;
-          Value.Integer IntegerKind.U8 0;
-          Value.Integer IntegerKind.U8 0;
-          Value.Integer IntegerKind.U8 0;
-          Value.Integer IntegerKind.U8 0;
-          Value.Integer IntegerKind.U8 0;
-          Value.Integer IntegerKind.U8 0;
-          Value.Integer IntegerKind.U8 0;
-          Value.Integer IntegerKind.U8 0;
-          Value.Integer IntegerKind.U8 0;
-          Value.Integer IntegerKind.U8 0;
-          Value.Integer IntegerKind.U8 0;
-          Value.Integer IntegerKind.U8 0;
-          Value.Integer IntegerKind.U8 0;
-          Value.Integer IntegerKind.U8 0;
-          Value.Integer IntegerKind.U8 0;
-          Value.Integer IntegerKind.U8 0;
-          Value.Integer IntegerKind.U8 0;
-          Value.Integer IntegerKind.U8 0;
-          Value.Integer IntegerKind.U8 0;
-          Value.Integer IntegerKind.U8 0;
-          Value.Integer IntegerKind.U8 0;
-          Value.Integer IntegerKind.U8 0;
-          Value.Integer IntegerKind.U8 0;
-          Value.Integer IntegerKind.U8 0;
-          Value.Integer IntegerKind.U8 0;
-          Value.Integer IntegerKind.U8 0;
-          Value.Integer IntegerKind.U8 0;
-          Value.Integer IntegerKind.U8 0;
-          Value.Integer IntegerKind.U8 0;
-          Value.Integer IntegerKind.U8 0;
-          Value.Integer IntegerKind.U8 0;
-          Value.Integer IntegerKind.U8 0;
-          Value.Integer IntegerKind.U8 0;
-          Value.Integer IntegerKind.U8 0;
-          Value.Integer IntegerKind.U8 0;
-          Value.Integer IntegerKind.U8 0;
-          Value.Integer IntegerKind.U8 0;
-          Value.Integer IntegerKind.U8 0;
-          Value.Integer IntegerKind.U8 0
-        ])
+        M.alloc (Value.Array (List.repeat
+          (Value.Integer IntegerKind.U8 0)
+          (Z.to_nat (((N.(Integer.value) / BLOCK_SIZE_IN_BYTES) + 1) * BLOCK_SIZE_IN_BYTES))))
       |) ]] in
       do~ [[
         M.if_ (|
